lean/LoVe/LoVe02_ProgramsAndTheorems_HomeworkSheet.lean
@@ -21,14 +21,18 @@ namespace LoVe
 end of a list. Your function should be defined by recursion and not using `++`
 (`List.append`). -/
 
-def snoc {α : Type} : List α → α → List α :=
-  sorry
+def snoc {α : Type} : List α → α → List α
+  | [], a' => [a']
+  | a :: as, a' => a :: snoc as a'
+
 
 /- 1.2 (1 point). Convince yourself that your definition of `snoc` works by
 testing it on a few examples. -/
 
 #eval snoc [1] 2
 -- invoke `#eval` or `#reduce` here
+#eval snoc [1, 2, 3] 4
+#eval snoc [] 1
 
 
 /- ## Question 2 (6 points): Sum
@@ -36,8 +40,9 @@ testing it on a few examples. -/
 2.1 (3 points). Define a `sum` function that computes the sum of all the numbers
 in a list. -/
 
-def sum : List ℕ → ℕ :=
-  sorry
+def sum : List ℕ → ℕ
+  | []      => 0
+  | n :: ns => n + sum ns
 
 #eval sum [1, 12, 3]   -- expected: 16
 
@@ -51,5 +56,14 @@ def sum : List ℕ → ℕ :=
 Try to give meaningful names to your theorems. Use `sorry` as the proof. -/
 
 -- enter your theorem statements here
+
+theorem sum_snoc (ms : List ℕ) (n : ℕ) :
+  sum (snoc ms n) = n + sum ms := sorry
+
+theorem sum_append (ms ns : List ℕ) :
+  sum (ms ++ ns) = sum ms + sum ns := sorry
+
+theorem sum_reverse (ns : List ℕ) :
+  sum (reverse ns) = sum ns := sorry
 
 end LoVe
