lean/LoVe/LoVe02_ProgramsAndTheorems_Note.lean
@@ -1,0 +1,147 @@
+
+import LoVe.LoVelib
+
+/- # LoVe Note 2: Programs and Theorems -/
+
+set_option autoImplicit false
+set_option tactic.hygienic false
+
+namespace LoVe
+
+/- ## Type Definitions -/
+
+namespace MyNat
+
+inductive Nat : Type where
+  | zero : Nat
+  | succ : Nat → Nat
+
+#check Nat
+#check Nat.zero
+#check Nat.succ
+#check Nat.succ .zero
+
+#print Nat
+
+end MyNat
+
+inductive AExp : Type where
+  | num : ℤ → AExp
+  | var : String → AExp
+  | add : AExp → AExp → AExp
+  | sub : AExp → AExp → AExp
+  | mul : AExp → AExp → AExp
+  | div : AExp → AExp → AExp
+
+#check AExp
+#check AExp.num
+#check AExp.num (-5)
+#check AExp.add
+#check AExp.add (.var "x") (.num 3)
+
+#print AExp
+#print AExp.add
+
+
+namespace MyList
+
+inductive List (α : Type) where
+  | nil   : List α
+  | cons  : α → List α → List α
+
+#check List.nil
+#check List.cons
+#check List.cons 1 .nil
+
+end MyList
+
+/- ## Function Definition -/
+
+def fib : ℕ → ℕ
+  | 0     => 0
+  | 1     => 1
+  | n + 2 => fib (n + 1) + fib n
+
+def add : ℕ → ℕ → ℕ
+  | m, .zero    => m
+  | m, .succ n  => .succ (add m n)
+
+#eval add 2 7
+#reduce add 2 7
+
+def mul : ℕ → ℕ → ℕ
+  | _, .zero    => .zero
+  | m, .succ n  => add m (mul m n)
+
+#eval mul 2 7
+
+def power : ℕ → ℕ → ℕ
+  | _, .zero    => 1
+  | m, .succ n  => mul m (power m n)
+
+#eval power 3 0
+#eval power 3 3
+
+def powerParam (m : ℕ) : ℕ → ℕ
+  | .zero     => 1
+  | .succ n   => mul m (powerParam m n)
+
+def iter (α : Type) (z : α) (f : α → α) : ℕ → α
+  | .zero     => z
+  | .succ n   => f (iter α z f n)
+
+def powerIter (m n : ℕ) : ℕ :=
+  iter ℕ 1 (mul m) n
+
+#eval powerParam 3 0
+#eval powerParam 3 4
+
+#eval powerIter 3 0
+#eval powerIter 3 4
+
+
+def eval (env : String → ℤ) : AExp → ℤ
+  | .num i      => i
+  | .var x      => env x
+  | .add e₁ e₂  => eval env e₁ + eval env e₂
+  | .sub e₁ e₂  => eval env e₁ - eval env e₂
+  | .mul e₁ e₂  => eval env e₁ * eval env e₂
+  | .div e₁ e₂  => eval env e₁ / eval env e₂
+
+#eval eval (fun _ ↦ 7) (.div (.var "y") (.num 0))
+#eval eval (fun _ ↦ 7) (.div (.var "y") (.num 2))
+
+
+def append (α : Type) : List α → List α → List α
+  | .nil,       ys => ys
+  | .cons x xs, ys => .cons x (append α xs ys)
+
+#eval append ℕ [3, 1] [4, 1, 5]
+#eval append _ [3, 1] [4, 1, 5]
+
+def appendImplicit {α : Type} : List α → List α → List α
+  | .nil,       ys => ys
+  | .cons x xs, ys => .cons x (appendImplicit xs ys)
+
+#eval appendImplicit [3, 1] [4, 1, 5]
+#eval @appendImplicit ℕ [3, 1] [4, 1, 5]
+#eval @appendImplicit _ [3, 1] [4, 1, 5]
+
+def appendPretty {α : Type} : List α → List α → List α
+  | [],       ys => ys
+  | x :: xs,  ys => x :: appendPretty xs ys
+
+def reverse {α : Type} : List α → List α
+  | []        => []
+  | x :: xs   => reverse xs ++ [x]
+
+/- Theorem Statements -/
+
+theorem add_comm (m n) :
+  add m n = add n m :=
+  sorry
+
+
+
+
+end LoVe
